README.md
@@ -1,0 +1,8 @@
+# comb_exp
+
+## build
+
+```sh
+coq_makefile -f _CoqProject -o Makefile
+make
+```
